SlowTest/ADT-int.dfy
@@ -1,0 +1,331 @@
+module ADT {
+  export Basic
+    provides
+      AbInt, I2A, A2D, Props_adt_dt_lt,
+      AbLt, AbAdd, AbSub, AbDiv2, AbDiv, AbLeq, AbLtLt, AbLeqLt,
+      /* Properties */
+      Props_one_in_bound_p2, Props_2is1add1,
+
+      /* Less Than */
+      Props_lt_gt_eq_p2, Props_lt2leq_p2, Props_leq2lt_p2,
+      Props_lt_addition_p3, Props_lt_transitive_p3,
+      Props_lt_add_notneg_p3,
+
+      /* Addition */
+      Props_add_commutative_p2, Props_add_associative_p3, Props_add_addition_p3, Props_add_identity_p1,
+      Props_add_lt_is_lt_p4, Props_add_notneg_is_leq_p3, Props_add_pos_is_lt_p2, Props_add_pos_is_pos_p2,
+      Props_add2sub_p3, Props_add_sub_is_add_p3, Props_add_sub_is_orig_p2,
+
+      /* Divide 2 */
+      Props_div_pos1_p1, Props_div_pos2_p1, Props_div_zero_p1, Props_div_lt_p1, Props_div_leq_p2, Props_div_add1_leq_p1
+    reveals
+      Nat, I0, I1, I2,
+      AbPos, AbIsZero, AbNotNeg
+
+  type AbInt(!new)(==) = int // (!new): generic type, not a class type
+  datatype Nat = Z | S(Nat)
+  const I0 : AbInt := I2A(0)
+  const I1 : AbInt := I2A(1)
+  const I2 : AbInt := I2A(2)
+
+  function method I2A (n: int) : (AbInt) { n }
+  function method A2D (a: AbInt) : Nat
+  lemma Props_adt_dt_lt (x: AbInt, y: AbInt)
+    requires AbLt(x, y)
+    ensures A2D(x) < A2D(y)
+
+  predicate AbIsZero (n: AbInt) { n == I0 }
+  predicate AbPos (n: AbInt) { AbLt(I0, n) }
+  predicate AbNotNeg (n: AbInt) { AbLeq(I0, n) }
+
+  function method AbLt (n: AbInt, m: AbInt) : bool { n < m }
+  function method AbAdd (n: AbInt, m: AbInt) : AbInt { n + m }
+  function method AbSub (n: AbInt, m: AbInt) : AbInt { n - m }
+  function method AbDiv2 (n: AbInt): (r: AbInt)
+    ensures AbLeq(AbAdd(r, r), n)
+    { n / 2 }
+  function method AbDiv (n: AbInt, m: AbInt) : AbInt
+    requires m != I0
+    { n / m }
+
+  function method AbLeq (n: AbInt, m: AbInt) : (r: bool)
+    ensures AbLeq(n, m) <==> AbLt(n, m) || n == m
+    { n <= m }
+  function method AbLtLt (x: AbInt, l: AbInt, h: AbInt): (r: bool)
+    ensures AbLtLt(x, l, h) <==> AbLt(l, x) && AbLt(x, h)
+    { l < x && x < h }
+  function method AbLeqLt(x: AbInt, l: AbInt, h: AbInt): (r: bool)
+    ensures AbLeqLt(x, l, h) <==> AbLeq(l, x) && AbLt(x, h)
+    { l <= x < h }
+
+  /* Properties */
+  
+  lemma Props_2is1add1 ()
+    ensures I2 == AbAdd(I1, I1)
+    { }
+  lemma Props_one_in_bound_p2 (a: AbInt, x: AbInt)
+    ensures AbLeq(a, x) && AbLt(x, AbAdd(a, I1)) ==> x == a
+    { }
+  
+  lemma Props_lt_gt_eq_p2 (x: AbInt, y: AbInt)
+    // x < y or x < y or x == y
+    // ensures AbLt(x, y) || AbLt(y, x) || x == y
+    ensures AbLt(x, y) <==> !AbLeq(y, x)
+    { }
+  lemma Props_lt2leq_p2 (x: AbInt, y: AbInt)
+    // x < y <==> x + 1 <= y <==> x <= y - 1
+    ensures AbLt(x, y) ==> AbLeq(AbAdd(x, I1), y)
+    ensures AbLt(x, y) ==> AbLeq(x, AbSub(y, I1))
+
+  lemma Props_leq2lt_p2 (x: AbInt, y: AbInt)
+    // x <= y <==> x - 1 < y <==> x < y + 1
+    ensures AbLeq(x, y) ==> AbLt(AbSub(x, I1), y)
+    ensures AbLeq(x, y) ==> AbLt(x, AbAdd(y, I1))
+    { }
+
+  lemma Props_lt_addition_p3 (x: AbInt, y: AbInt, a: AbInt)
+    // x < y ==> x + a < y + a
+    ensures AbLt(x, y) ==> AbLt(AbAdd(x, a), AbAdd(y, a))
+    { }
+  lemma Props_lt_transitive_p3 (x: AbInt, y: AbInt, z: AbInt)
+    // x < y < z
+    ensures AbLt(x, y) && AbLt(y, z) ==> AbLt(x, z)
+    { }
+  lemma Props_lt_add_notneg_p3 (x: AbInt, y: AbInt, a: AbInt)
+    // x + a < y ==> x < y
+    ensures AbNotNeg(a) && AbLt(AbAdd(x, a), y) ==> AbLt(x, y)
+    { }
+
+  lemma Props_add_commutative_p2 (x: AbInt, y: AbInt)
+    // x + y == y + x
+    ensures AbAdd(x, y) == AbAdd(y, x)
+    { }
+  lemma Props_add_associative_p3 (x: AbInt, y: AbInt, z: AbInt)
+    // (x + y) + z == x + (y + z)
+    ensures AbAdd(AbAdd(x, y), z) == AbAdd(x, AbAdd(y, z))
+    { }
+  lemma Props_add_addition_p3 (x: AbInt, y: AbInt, a: AbInt)
+    // x + a == y + a ==> x == y
+    ensures AbAdd(x, a) == AbAdd(y, a) <==> x == y
+    { }
+  lemma Props_add_identity_p1 (x: AbInt)
+    // x + 0 == 0 + x == x
+    ensures AbAdd(x, I0) == AbAdd(I0, x) == x
+    { }
+
+  lemma Props_add_lt_is_lt_p4 (x: AbInt, y: AbInt, a: AbInt, b: AbInt)
+    // x = y + a && a < b ==> x < y + b
+    ensures x == AbAdd(y, a) && AbLt(a, b) ==> AbLt(x, AbAdd(y, b))
+    { }
+  lemma Props_add_notneg_is_leq_p3 (x: AbInt, y: AbInt, a: AbInt)
+    //  x + NotNeg == y ==> x <= y
+    ensures AbNotNeg(a) && (AbAdd(x, a) == y) ==> AbLeq(x, y)
+    { }
+  lemma Props_add_pos_is_lt_p2 (x: AbInt, a: AbInt)
+    // x < x + Positive (x + Positive != x)
+    ensures AbPos(a) ==> AbLt(x, AbAdd(x, a)); // AbAdd(x, a) != x
+    { }
+  lemma Props_add_pos_is_pos_p2 (x: AbInt, a: AbInt)
+    // NotNeg + Positive is Positive
+    requires AbNotNeg(x)
+    ensures AbPos(a) ==> AbPos(AbAdd(x, a))
+    { }
+  lemma Props_add2sub_p3 (x: AbInt, y: AbInt, z: AbInt)
+    // x + y == z ==> x = z - y && y = z - x
+    ensures AbAdd(x, y) == z <==> AbSub(z, y) == x && AbSub(z, x) == y
+    { }
+  lemma Props_add_sub_is_orig_p2 (x: AbInt, y: AbInt)
+    // x + y == z ==> x = z - y && y = z - x
+    ensures AbAdd(AbSub(x, y), y) == x
+    ensures AbSub(AbAdd(x, y), y) == x
+    { }
+  lemma Props_add_sub_is_add_p3 (x: AbInt, a: AbInt, b: AbInt)
+    // x + b + (a - b) == x + a
+    ensures AbAdd(AbAdd(x, b), AbSub(a, b)) == AbAdd(x, a)
+    { }
+
+  lemma Props_div_pos2_p1 (x: AbInt)
+    // x / 2 is Positive <==> x >= 2
+    ensures AbLeq(I2, x) <==> AbPos(AbDiv2(x))
+    { }
+  lemma Props_div_pos1_p1 (x: AbInt)
+    // (x + 1) / 2 is Positive <==> x >= 1
+    ensures AbLeq(I1, x) <==> AbPos(AbDiv2(AbAdd(x, I1)))
+    { }
+  lemma Props_div_zero_p1 (x: AbInt)
+    // 1 / 2 == 0 and 0 / 2 == 0
+    ensures x == I0 || x == I1 <==> AbDiv2(x) == I0
+    { }
+  lemma Props_div_lt_p1 (x: AbInt)
+    // I2 <= x ==> x / 2 < x
+    ensures AbLeq(I2, x) ==> AbLt(AbDiv2(x), x)
+    { }
+  lemma Props_div_leq_p2 (x: AbInt, y: AbInt)
+    // y <= x ==> (x + y) / 2 <= x
+    ensures AbLeq(y, x) ==> AbLeq(AbDiv2(AbAdd(x, y)), x)
+    { }
+  lemma Props_div_add1_leq_p1 (x: AbInt)
+    // 1 <= x ==> (x / 2 + 1) <= x
+    ensures AbLeq(I1, x) ==> AbLeq(AbAdd(AbDiv2(x), I1), x)
+    { }
+}
+
+module ADT_Int
+{
+  import opened ADT`Basic
+
+  // Note: Props_notneg () might be an assumption
+  lemma Props_notneg ()
+    ensures forall x :: AbNotNeg(x)
+  // Note: Props_pos () might be an assumption
+  lemma Props_pos (x: AbInt)
+    ensures AbPos(x)
+
+  lemma Props_one_in_bound ()
+    ensures forall a, x :: AbLeqLt(x, a, AbAdd(a, I1)) ==> x == a
+    { forall a, x { Props_one_in_bound_p2(a, x); } }
+  
+  lemma Props_one_in_bound_p1 (a: AbInt)
+    ensures forall x :: AbLeqLt(x, a, AbAdd(a, I1)) ==> x == a
+    { forall x { Props_one_in_bound_p2(a, x); } }
+  
+  lemma Props_lt_gt_eq ()
+    // x < y or x < y or x == y
+    ensures forall x, y :: AbLt(x, y) <==> !AbLeq(y, x)
+    ensures forall x, y :: AbLt(x, y) <==> !(AbLt(y, x) || y == x)
+    { forall x, y { Props_lt_gt_eq_p2(x, y); } }
+  lemma Props_lt_gt_eq_px (x: AbInt)
+    // x < y or x < y or x == y
+    ensures forall y :: AbLt(x, y) <==> !AbLeq(y, x)
+    ensures forall y :: AbLt(x, y) <==> !(AbLt(y, x) || y == x)
+    { forall y { Props_lt_gt_eq_p2(x, y); } }
+  lemma Props_lt_gt_eq_py (y: AbInt)
+    // x < y or x < y or x == y
+    ensures forall x :: AbLt(x, y) <==> !AbLeq(y, x)
+    ensures forall x :: AbLt(x, y) <==> !(AbLt(y, x) || y == x)
+    { forall x { Props_lt_gt_eq_p2(x, y); } }
+  
+  lemma Props_lt2leq ()
+    // x < y <==> x + 1 <= y <==> x <= y - 1
+    ensures forall x, y :: AbLt(x, y) ==> AbLeq(AbAdd(x, I1), y)
+    ensures forall x, y :: AbLt(x, y) ==> AbLeq(x, AbSub(y, I1))
+    { forall x, y { Props_lt2leq_p2(x, y); } }
+  
+  lemma Props_leq2lt ()
+    ensures forall x, y :: AbLeq(x, y) ==> AbLt(AbSub(x, I1), y)
+    ensures forall x, y :: AbLeq(x, y) ==> AbLt(x, AbAdd(y, I1))
+    { forall x, y { Props_leq2lt_p2(x, y); } }
+
+  lemma Props_lt_addition ()
+    // x < y ==> x + a < y + a
+    ensures forall x, y, a :: AbLt(x, y) ==> AbLt(AbAdd(x, a), AbAdd(y, a))
+    { forall x, y, a { Props_lt_addition_p3(x, y, a); } }
+  lemma Props_lt_transitive ()
+    // x < y < z
+    ensures forall x, y, z :: AbLt(x, y) && AbLt(y, z) ==> AbLt(x, z)
+    { forall x, y, z {Props_lt_transitive_p3(x, y, z); } }
+  lemma Props_lt_add_notneg ()
+    // x + a < y ==> x < y
+    ensures forall x, y, a :: AbNotNeg(a) && AbLt(AbAdd(x, a), y) ==> AbLt(x, y)
+    { forall x, y, a { Props_lt_add_notneg_p3(x, y, a); } }
+
+  lemma Props_add_commutative ()
+    // x + y == y + x
+    ensures forall x, y :: AbAdd(x, y) == AbAdd(y, x)
+    { forall x, y { Props_add_commutative_p2(x, y); } }
+  lemma Props_add_associative ()
+    // (x + y) + z == x + (y + z)
+    ensures forall x, y, z :: AbAdd(AbAdd(x, y), z) == AbAdd(x, AbAdd(y, z))
+    { forall x, y, z { Props_add_associative_p3(x, y, z); } }
+  lemma Props_add_addition ()
+    // x + a == y + a ==> x == y
+    ensures forall x, y, a :: AbAdd(x, a) == AbAdd(y, a) <==> x == y
+    { forall x, y, a { Props_add_addition_p3(x, y, a); } }
+  lemma Props_add_identity ()
+    // x + 0 == 0 + x == x
+    ensures forall x :: AbAdd(x, I0) == AbAdd(I0, x) == x
+    { forall x { Props_add_identity_p1(x); } }
+
+  lemma Props_add_lt_is_lt ()
+    // x = y + a && a < b ==> x < y + b
+    ensures forall x, y, a, b :: x == AbAdd(y, a) && AbLt(a, b) ==> AbLt(x, AbAdd(y, b))
+    { forall x, y, a, b { Props_add_lt_is_lt_p4(x, y, a, b); } }
+  lemma Props_add_notneg_is_leq ()
+    //  x + NotNeg == y ==> x <= y
+    ensures forall x, y, a :: AbNotNeg(a) && (AbAdd(x, a) == y) ==> AbLeq(x, y)
+    { forall x, y, a { Props_add_notneg_is_leq_p3(x, y, a); } }
+  lemma Props_add_pos_is_lt ()
+    // x < x + Positive (x + Positive != x)
+    ensures forall x, a :: AbPos(a) ==> AbLt(x, AbAdd(x, a)); // AbAdd(x, a) != x
+    { forall x, a { Props_add_pos_is_lt_p2(x, a); } }
+  lemma Props_add_pos_is_pos ()
+    // NotNeg + Positive is Positive
+    requires forall x :: AbNotNeg(x)
+    ensures forall x, a :: AbPos(a) ==> AbPos(AbAdd(x, a))
+    { forall x, a { Props_add_pos_is_pos_p2(x, a); } }
+  lemma Props_add2sub ()
+    // x + y == z ==> x = z - y && y = z - x
+    ensures forall x, y, z :: AbAdd(x, y) == z <==> AbSub(z, y) == x && AbSub(z, x) == y
+    { forall x, y, z { Props_add2sub_p3(x, y, z); } }
+  lemma Props_add_sub_is_orig ()
+    // x + y == z ==> x = z - y && y = z - x
+    ensures forall x, y :: AbAdd(AbSub(x, y), y) == x
+    ensures forall x, y :: AbSub(AbAdd(x, y), y) == x
+    { forall x, y { Props_add_sub_is_orig_p2(x, y); } }
+  lemma Props_add_sub_is_add ()
+    // x + b + (a - b) == x + a
+    ensures forall x, a, b :: AbAdd(AbAdd(x, b), AbSub(a, b)) == AbAdd(x, a)
+    { forall x, a, b { Props_add_sub_is_add_p3(x, a, b); } }
+
+  lemma Props_div_pos2 ()
+    // x / 2 is Positive <==> x >= 2
+    ensures forall x :: AbLeq(I2, x) <==> AbPos(AbDiv2(x))
+    { forall x { Props_div_pos2_p1(x); } }
+  lemma Props_div_pos1 ()
+    // (x + 1) / 2 is Positive <==> x >= 1
+    ensures forall x :: AbLeq(I1, x) <==> AbPos(AbDiv2(AbAdd(x, I1)))
+    { forall x { Props_div_pos1_p1(x); } }
+  lemma Props_div_zero ()
+    // 1 / 2 == 0 and 0 / 2 == 0
+    ensures forall x :: x == I0 || x == I1 <==> AbDiv2(x) == I0
+    { forall x { Props_div_zero_p1(x); } }
+  lemma Props_div_lt ()
+    // I2 <= x ==> x / 2 < x
+    ensures forall x :: AbLeq(I2, x) ==> AbLt(AbDiv2(x), x)
+    { forall x { Props_div_lt_p1(x); } }
+  lemma Props_div_leq ()
+    // y <= x ==> (x + y) / 2 <= x
+    ensures forall x, y :: AbLeq(y, x) ==> AbLeq(AbDiv2(AbAdd(x, y)), x)
+    { forall x, y { Props_div_leq_p2(x, y); } }
+  lemma Props_div_add1_leq ()
+    // 1 <= x ==> (x / 2 + 1) <= x
+    ensures forall x :: AbLeq(I1, x) ==> AbLeq(AbAdd(AbDiv2(x), I1), x)
+    { forall x { Props_div_add1_leq_p1(x); } }
+}
+
+module ADT_Set {
+  import opened ADT`Basic
+
+  function method AbSetLen(s: set<AbInt>) : (l: AbInt)
+
+  // Set generation: lo <= x < hi
+  // experiment with more trigger options
+  function method AbBoundSet(lo: AbInt, hi: AbInt): (S: set<AbInt>)
+    ensures AbSetLen(S) == AbSub(hi, lo)
+    ensures forall x :: AbLeq(lo, x) && AbLt(x, hi) <==> x in S
+    // Try not to assign every element with AbAdd()
+    // ensures S == set x | 0 <= x < len :: AbAdd(lo, int2adt(x))
+
+  lemma Set_Props_len ()
+    ensures forall x :: AbLeq(I0, AbSetLen(x))
+  
+  lemma Set_Props_len_empty ()
+    ensures forall x :: AbSetLen(x) == I0 <==> x == {}
+  
+  lemma Set_Props_len_singlton ()
+    ensures forall x: AbInt :: AbSetLen({x}) == I1
+
+  lemma Set_Props_len_element ()
+    ensures forall x: AbInt, A: set<AbInt> :: x in A ==> AbSetLen(A) == AbAdd(AbSetLen(A - {x}), I1)
+
+}
