SlowTest/ADT-seq.dfy
@@ -1,0 +1,438 @@
+include "ADT-int.dfy"
+module ADT_Seq refines ADT {
+  export Basic 
+    provides AbSeq,
+      AbSeqLen, AbSeqIndex, AbSeqConcat, AbSeqIn, AbSeqEmpty, AbSeqSingleton, AbSeqSlice,
+      AbSeqGetIdx, AbSeqRemove, AbSeqRemoveIdx, AbSeqUpdate, AbSeqInit,
+
+      Seq_Props_length_p1, Seq_Props_concat_length_p2,
+      Seq_Props_concat_in_p3, Seq_Props_concat_in_part2all_p3, Seq_Props_concat_in_all2part_p3,
+      Seq_Props_concat_index_part1_p3, Seq_Props_concat_index_part2_p3,
+      Seq_Props_concat_is_orig_p2,
+      Seq_Props_in_empty_p2, Seq_Props_in_non_empty_p2,
+      Seq_Props_in_idx_p2,
+      Seq_Props_slice_in_p4,
+      Seq_Props_index_props
+
+  import opened ADT_Int
+  type AbSeq<X(==)> = seq<X>
+  function method AbSeqLen<X> (s: AbSeq<X>) : AbInt { |s| }
+  function method AbSeqIndex<X> (i: AbInt, s: AbSeq<X>) : X
+    requires AbLeq(I0, i)
+    requires AbLt(i, AbSeqLen(s))
+    ensures AbSeqIn(AbSeqIndex(i, s), s)
+    { s[i] }
+
+  function method AbSeqConcat<X> (s1: AbSeq<X>, s2: AbSeq<X>) : AbSeq<X> { s1 + s2 }
+  function method AbSeqIn<X> (v: X, s: AbSeq<X>) : bool { v in s }
+
+  function method AbSeqEmpty<X> (): (s: AbSeq<X>)
+    ensures AbSeqLen(s) == I0
+    { [] }
+
+  function method AbSeqSingleton<X(!new)> (v: X): (s: AbSeq<X>)
+    ensures AbSeqLen(s) == I1
+    ensures AbLt(I0, I1) ==> AbSeqIndex(I0, s) == v
+    ensures AbSeqIn(v, s)
+    ensures forall x :: x != v ==> !AbSeqIn(x, s)
+    { [v] }
+
+  function method AbSeqSlice<X> (i: AbInt, j: AbInt, s: AbSeq<X>) : (s' : AbSeq<X>)
+    requires AbLeq(I0, i)
+    requires AbLeq(j, AbSeqLen(s))
+    requires AbLeq(i, j)
+    ensures AbSeqLen(s') == AbSub(j, i)
+    ensures forall x :: AbLeq(i, x) && AbLt(x, j) ==>
+      // precond begins
+      AbLeq(I0, x) ==> AbLt(x, AbSeqLen(s)) ==>
+      AbLeq(I0, AbSub(x, i)) ==> AbLt(AbSub(x, i), AbSeqLen(s')) ==>
+      // precond ends
+      AbSeqIndex(x, s) == AbSeqIndex(AbSub(x, i), s') // s[i..j] w/ s[i] and w/o s[j]
+    { s[i..j] }
+
+  function method AbSeqGetIdx<X>(v: X, s: AbSeq<X>) : (i: AbInt)
+    requires AbSeqIn(v, s)
+    ensures AbLeqLt(i, I0, AbSeqLen(s))
+    ensures AbSeqIndex(i, s) == v
+
+  function method AbSeqInit<X> (len: AbInt, func : AbInt --> X) : (s: AbSeq<X>)
+    requires forall i :: AbLeq(I0, i) && AbLt(i, len) ==> func.requires(i)
+    ensures AbSeqLen(s) == len
+    ensures forall i :: AbLeqLt(i, I0, len) ==>
+      AbSeqIndex(i, s) == func(i)
+
+  function method AbSeqRemove<X(!new)> (v: X, s: AbSeq<X>): (s': AbSeq<X>)
+    requires AbSeqIn(v, s)
+    ensures AbSeqLen(s) == AbAdd(AbSeqLen(s'), I1)
+    ensures AbSeqLen(s') == AbSub(AbSeqLen(s), I1)
+    // ensures forall v :: AbSeqIn(v, s') ==> AbSeqIn(v, s)
+    ensures var k := AbSeqGetIdx(v, s);
+      forall i :: // s[0, k) keeps
+        AbLeqLt(i, I0, k) ==>
+        // precond begins
+        AbLt(i, AbSeqLen(s)) ==>
+        AbLt(i, AbSeqLen(s')) ==>
+        // precond ends
+        AbSeqIndex(i, s) == AbSeqIndex(i, s')
+    ensures var k := AbSeqGetIdx(v, s);
+      forall i :: // s(k, |s|-1] keeps
+        AbLt(k, i) && AbLt(i, AbSeqLen(s')) ==>
+        // precond begins
+        AbLeq(I0, i) ==>
+        AbLt(I0, AbAdd(i, I1)) ==>
+        AbLt(AbAdd(i, I1), AbSeqLen(s)) ==>
+        // precond ends
+        AbSeqIndex(AbAdd(i, I1), s) == AbSeqIndex(i, s')
+  {
+    var k := AbSeqGetIdx(v, s);
+    AbSeqRemoveIdx(k, s)
+  }
+
+  function method AbSeqRemoveIdx<X(!new)> (k: AbInt, s: AbSeq<X>) : (s': AbSeq<X>)
+    requires AbLt(k, AbSeqLen(s))
+    requires AbLt(I0, k) || I0 == k
+    ensures AbSeqLen(s) == AbAdd(AbSeqLen(s'), I1)
+    ensures AbSeqLen(s') == AbSub(AbSeqLen(s), I1)
+    // ensures forall v :: AbSeqIn(v, s') ==> AbSeqIn(v, s)
+    ensures
+      forall i :: // s[0, k) keeps
+        AbLeqLt(i, I0, k) ==>
+        // precond begins
+        AbLt(i, AbSeqLen(s)) ==>
+        AbLt(i, AbSeqLen(s')) ==>
+        // precond ends
+        AbSeqIndex(i, s) == AbSeqIndex(i, s')
+    ensures
+      forall i :: // s(k, |s|-1] keeps
+        AbLt(k, i) && AbLt(i, AbSeqLen(s')) ==>
+        // precond begins
+        AbLeq(I0, i) ==>
+        AbLt(I0, AbAdd(i, I1)) ==>
+        AbLt(AbAdd(i, I1), AbSeqLen(s)) ==>
+        // precond ends
+        AbSeqIndex(AbAdd(i, I1), s) == AbSeqIndex(i, s')
+  {
+    var len := AbSeqLen(s);
+    var half1 := AbSeqSlice(I0, k, s);
+    Props_add2sub ();
+    Props_add_identity ();
+    Props_notneg ();
+    assume AbPos(I1); // Props_pos (I1);
+    Props_add_pos_is_lt ();
+    Props_lt_transitive ();
+    if AbLt(AbAdd(k, I1), len) then
+      var half2 := AbSeqSlice(AbAdd(k, I1), len, s);
+      // var s':= AbSeqConcat(half1, half2);
+      Seq_Props_concat_length_p2 (half1, half2);
+      Props_add_associative ();
+      Props_lt_addition ();
+      Seq_Props_concat_index_part1<X> ();
+      // assert forall i :: // s[0, k) keeps
+      //   (AbLt(I0, i) || I0 == i) &&
+      //   AbLt(i, k) ==> 
+      //   AbSeqIndex(i, s) == AbSeqIndex(i, s');
+      Props_add_commutative ();
+      Seq_Props_concat_index_part2<X> ();
+      // assert forall i :: // s(k, |s|-1] keeps
+      //   (AbLt(k, i) || i == k) &&
+      //   AbLt(i, AbSeqLen(s')) ==>
+      //   AbSeqIndex(AbAdd(i, I1), s) == 
+      //   AbSeqIndex(i, s');
+      Seq_Props_slice_in<X> ();
+      Seq_Props_concat_in<X> ();
+      // assert forall v :: AbSeqIn(v, s') ==> AbSeqIn(v, s);
+      AbSeqConcat(half1, half2)
+    else
+      Props_lt_gt_eq ();
+      Props_lt2leq ();
+      Seq_Props_slice_in<X> ();
+      // assert forall v :: AbSeqIn(v, half1) ==> AbSeqIn(v, s);
+      // assert forall i :: // s[0, k) keeps
+      //   (AbLt(I0, i) || I0 == i) &&
+      //   AbLt(i, AbSub(len, I1)) ==> 
+      //   AbSeqIndex(i, s) == AbSeqIndex(i, s');
+      // assert forall i :: // s(k, |s|-1] keeps
+      //   (AbLt(k, i) || i == k) &&
+      //   AbLt(i, AbSeqLen(s')) ==>
+      //   AbSeqIndex(AbAdd(i, I1), s) == AbSeqIndex(i, s');
+      half1
+  }
+
+  function method AbSeqUpdate<X> (k: AbInt, v: X, s: AbSeq<X>): (s': AbSeq<X>)
+    requires AbLt(k, AbSeqLen(s))
+    requires AbLeq(I0, k)
+    ensures AbSeqLen(s) == AbSeqLen(s')
+    ensures AbSeqIndex(k, s') == v
+    ensures
+      forall i :: // s[0, k) keeps
+        AbLeqLt(i, I0, k) ==>
+        // precond begins
+        AbLt(i, AbSeqLen(s)) ==>
+        AbLt(i, AbSeqLen(s')) ==>
+        // precond ends
+        AbSeqIndex(i, s) == AbSeqIndex(i, s')
+    ensures
+      forall i :: // s(k, |s|-1] keeps
+        AbLt(k, i) && AbLt(i, AbSeqLen(s')) ==>
+        // precond begins
+        AbLeq(I0, i) ==>
+        AbLt(i, AbSeqLen(s)) ==>
+        // precond ends
+        AbSeqIndex(i, s) == AbSeqIndex(i, s')
+  {
+    var len := AbSeqLen(s);
+    var half1 := AbSeqSlice(I0, k, s);
+    Props_add2sub ();
+    Props_add_identity ();
+    Props_notneg ();
+    assume AbPos(I1); // Props_pos (I1);
+    Props_add_pos_is_lt ();
+    Props_lt_transitive ();
+    Props_add_commutative ();
+    if AbLt(AbAdd(k, I1), len) then
+      var half2 := AbSeqSlice(AbAdd(k, I1), len, s);
+      var half1' := AbSeqConcat(half1, AbSeqSingleton(v));
+      Seq_Props_concat_length_p2 (half1, AbSeqSingleton(v));
+      Seq_Props_concat_length_p2 (half1', half2);
+      // var s' := AbSeqConcat(half1', half2);
+      // assert len == AbSeqLen(s');
+      Props_lt_addition ();
+      Seq_Props_concat_index_part1<X> ();
+      // assert forall i :: // s[0, k) keeps
+      //   (AbLt(I0, i) || I0 == i) &&
+      //   AbLt(i, k) ==>
+      //   AbSeqIndex(i, s) == AbSeqIndex(i, s');
+      // Seq_Props_concat_is_orig<X> ();
+      Seq_Props_concat_is_orig_p2 (AbAdd(k, I1), s);
+      Seq_Props_concat_index_part2<X> ();
+      // Seq_Props_concat_index_part2_param (I0, half1, AbSeqSingleton(v));
+      // assert AbSeqIndex(k, half1') == v;
+      
+      // assert forall i :: // s(k, |s|-1] keeps
+      //   AbLt(k, i) && AbLt(i, AbSeqLen(s)) ==>
+      //   AbSeqIndex(i, s) == AbSeqIndex(AbSub(i, AbAdd(k, I1)), half2);
+      // assert forall i :: // s(k, |s|-1] keeps
+      //   AbLt(k, i) &&
+      //   AbLt(i, AbSeqLen(s')) ==>
+      //   AbSeqIndex(i, s) == AbSeqIndex(i, s');
+      AbSeqConcat(half1', half2)
+    else
+      Props_lt_gt_eq_p2 (AbAdd(k, I1), len);
+      Props_lt2leq ();
+      // var s' := AbSeqConcat(half1, AbSeqSingleton(v));
+      Seq_Props_concat_length_p2 (half1, AbSeqSingleton(v));
+      // assert AbSeqLen(s') == len;
+      Seq_Props_concat_index_part1<X> ();
+      // assert forall i :: // s[0, k) keeps
+      //   (AbLt(I0, i) || I0 == i) &&
+      //   AbLt(i, k) ==>
+      //   AbSeqIndex(i, s) == AbSeqIndex(i, s');
+      // assert forall i :: // s(k, |s|-1] keeps
+      //   AbLt(k, i) &&
+      //   AbLt(i, AbSeqLen(s')) ==>
+      //   AbSeqIndex(i, s) == AbSeqIndex(i, s');
+      Seq_Props_concat_index_part2<X> ();
+      // assert AbSeqIndex(k, s') == v;
+      AbSeqConcat(half1, AbSeqSingleton(v))
+}
+
+  lemma Seq_Props_length_p1<X> (s: AbSeq<X>) // |s| >= 0
+    ensures forall s: AbSeq<X> :: AbLeq(I0, AbSeqLen(s))
+    {}
+  lemma Seq_Props_length<X> () // |s| >= 0
+    ensures forall s: AbSeq<X> :: AbLeq(I0, AbSeqLen(s))
+    { forall s { Seq_Props_length_p1<X> (s); } }
+
+  lemma Seq_Props_concat_length_p2<X> (s1: AbSeq<X>, s2: AbSeq<X>) // |s1 + s2| == |s1| + |s2|
+    ensures AbSeqLen(AbSeqConcat(s1, s2)) == AbAdd(AbSeqLen(s1), AbSeqLen(s2))
+    { }
+  lemma Seq_Props_concat_length<X> () // |s1 + s2| == |s1| + |s2|
+    ensures forall s1: AbSeq<X>, s2: AbSeq<X> :: AbSeqLen(AbSeqConcat(s1, s2)) == AbAdd(AbSeqLen(s1), AbSeqLen(s2))
+    { forall s1, s2 { Seq_Props_concat_length_p2<X>(s1, s2); } }
+  
+  lemma Seq_Props_concat_in_p3<X> (x: X, s1: AbSeq<X>, s2: AbSeq<X>) // x in s1 || x in s2 <==> x in s1 + s2
+    ensures AbSeqIn(x, s1) || AbSeqIn(x, s2) <==> AbSeqIn(x, AbSeqConcat(s1, s2))
+    { }
+  lemma Seq_Props_concat_in<X> () // x in s1 || x in s2 <==> x in s1 + s2
+    ensures forall x: X, s1: AbSeq<X>, s2: AbSeq<X> :: AbSeqIn(x, s1) || AbSeqIn(x, s2) <==> AbSeqIn(x, AbSeqConcat(s1, s2))
+    { forall x, s1, s2 { Seq_Props_concat_in_p3<X>(x, s1, s2); } }
+
+  lemma Seq_Props_concat_in_part2all_p3<X> (x: X, s1: AbSeq<X>, s2: AbSeq<X>)
+    // x in s1 ==> x in s1 + s2
+    ensures AbSeqIn(x, s1) ==> AbSeqIn(x, AbSeqConcat(s1, s2))
+    // x in s2 ==> x in s1 + s2
+    ensures AbSeqIn(x, s2) ==> AbSeqIn(x, AbSeqConcat(s1, s2))
+    { }
+  lemma Seq_Props_concat_in_part2all<X> ()
+    // x in s1 ==> x in s1 + s2
+    ensures forall x: X, s1: AbSeq<X>, s2: AbSeq<X> :: AbSeqIn(x, s1) ==> AbSeqIn(x, AbSeqConcat(s1, s2))
+    // x in s2 ==> x in s1 + s2
+    ensures forall x: X, s1: AbSeq<X>, s2: AbSeq<X> :: AbSeqIn(x, s2) ==> AbSeqIn(x, AbSeqConcat(s1, s2))
+    { forall x, s1, s2 { Seq_Props_concat_in_part2all_p3<X>(x, s1, s2); } }
+
+  lemma Seq_Props_concat_in_all2part_p3<X> (x: X, s1: AbSeq<X>, s2: AbSeq<X>)
+    // x in s1 + s2 && x !in s1 ==> x in s2
+    ensures AbSeqIn(x, AbSeqConcat(s1, s2)) && !AbSeqIn(x, s1) ==> AbSeqIn(x, s2)
+    // x in s1 + s2 && x !in s2 ==> x in s1
+    ensures AbSeqIn(x, AbSeqConcat(s1, s2)) && !AbSeqIn(x, s2) ==> AbSeqIn(x, s1)
+    { }
+  lemma Seq_Props_concat_in_all2part<X> ()
+    // x in s1 + s2 && x !in s1 ==> x in s2
+    ensures forall x: X, s1: AbSeq<X>, s2: AbSeq<X> :: AbSeqIn(x, AbSeqConcat(s1, s2)) && !AbSeqIn(x, s1) ==> AbSeqIn(x, s2)
+    // x in s1 + s2 && x !in s2 ==> x in s1
+    ensures forall x: X, s1: AbSeq<X>, s2: AbSeq<X> :: AbSeqIn(x, AbSeqConcat(s1, s2)) && !AbSeqIn(x, s2) ==> AbSeqIn(x, s1)
+    { forall x, s1, s2 { Seq_Props_concat_in_all2part_p3<X>(x, s1, s2); } }
+
+  lemma Seq_Props_concat_index_part1_p3<X> (i: AbInt, s1: AbSeq<X>, s2: AbSeq<X>)
+    ensures AbLeqLt(i, I0, AbSeqLen(s1)) ==> // 0 <= i < |s1|
+    AbLt(i, AbSeqLen(AbSeqConcat(s1, s2))) ==> // i < |s1| < |s1 + s2|
+    AbSeqIndex(i, s1) == AbSeqIndex(i, AbSeqConcat(s1, s2))
+    { }
+  lemma Seq_Props_concat_index_part1<X> ()
+    ensures forall i: AbInt, s1: AbSeq<X>, s2: AbSeq<X> ::
+    AbLeqLt(i, I0, AbSeqLen(s1)) ==> // 0 <= i < |s1|
+    AbLt(i, AbSeqLen(AbSeqConcat(s1, s2))) ==> // i < |s1| < |s1 + s2|
+    AbSeqIndex(i, s1) == AbSeqIndex(i, AbSeqConcat(s1, s2))
+    { forall i, s1, s2 { Seq_Props_concat_index_part1_p3<X>(i, s1, s2); } }
+
+  lemma Seq_Props_concat_index_part2_p3<X> (i: AbInt, s1: AbSeq<X>, s2: AbSeq<X>)
+    ensures AbLeq(I0, AbAdd(i, AbSeqLen(s1))) ==> // 0 <= i + |s1|
+      (AbLt(i, AbSeqLen(s2)) ==> AbLt(AbAdd(i, AbSeqLen(s1)), AbSeqLen(AbSeqConcat(s1, s2)))) ==> // i + |s1| < |s1 + s2|
+      AbLeqLt(i, I0, AbSeqLen(s2)) ==>
+      AbSeqIndex(i, s2) == AbSeqIndex(AbAdd(i, AbSeqLen(s1)), AbSeqConcat(s1, s2))
+    { }
+  lemma Seq_Props_concat_index_part2<X> ()
+    ensures forall i: AbInt, s1: AbSeq<X>, s2: AbSeq<X> ::
+      AbLeq(I0, AbAdd(i, AbSeqLen(s1))) ==> // 0 <= i + |s1|
+      (AbLt(i, AbSeqLen(s2)) ==> AbLt(AbAdd(i, AbSeqLen(s1)), AbSeqLen(AbSeqConcat(s1, s2)))) ==> // i + |s1| < |s1 + s2|
+      AbLeqLt(i, I0, AbSeqLen(s2)) ==>
+      AbSeqIndex(i, s2) == AbSeqIndex(AbAdd(i, AbSeqLen(s1)), AbSeqConcat(s1, s2))
+    { forall i, s1, s2 { Seq_Props_concat_index_part2_p3<X>(i, s1, s2); } }
+
+  lemma Seq_Props_concat_is_orig_p2<X> (i: AbInt, s: AbSeq<X>)
+    ensures AbLeqLt(i, I0, AbSeqLen(s)) ==> // 0 <= i < |s|
+      s == AbSeqConcat(AbSeqSlice(I0, i, s), AbSeqSlice(i, AbSeqLen(s), s))
+    { }
+  lemma Seq_Props_concat_is_orig<X> ()
+    ensures forall i: AbInt, s: AbSeq<X> ::
+      AbLeqLt(i, I0, AbSeqLen(s)) ==> // 0 <= i < |s|
+      s == AbSeqConcat(AbSeqSlice(I0, i, s), AbSeqSlice(i, AbSeqLen(s), s))
+    { forall i, s { Seq_Props_concat_is_orig_p2<X> (i, s); } }
+
+  lemma Seq_Props_in_empty_p2<X> (v: X, s: AbSeq<X>) // empty seq
+    ensures AbSeqLen(s) == I0 ==> !AbSeqIn(v, s)
+    { }
+  lemma Seq_Props_in_empty<X> () // empty seq
+    ensures forall v: X, s: AbSeq<X> :: AbSeqLen(s) == I0 ==> !AbSeqIn(v, s)
+    {forall v, s { Seq_Props_in_empty_p2<X>(v, s); } }
+
+  lemma Seq_Props_in_non_empty_p2<X> (v: X, s: AbSeq<X>) // i in s ==> |s| > 0
+    ensures AbSeqIn(v, s) ==> AbLt(I0, AbSeqLen(s))
+    { }
+  lemma Seq_Props_in_non_empty<X> () // i in s ==> |s| > 0
+    ensures forall v: X, s: AbSeq<X> :: AbSeqIn(v, s) ==> AbLt(I0, AbSeqLen(s))
+    {forall v, s { Seq_Props_in_non_empty_p2<X>(v, s); } }
+
+  lemma Seq_Props_in_idx_p2<X> (v: X, s: AbSeq<X>) // v in s ==> s[i] == v
+    ensures AbSeqIn(v, s) ==>
+      (exists i: AbInt :: AbLeqLt(i, I0, AbSeqLen(s)) && AbSeqIndex(i, s) == v )
+  // NOTE: NEED PROVE
+  lemma Seq_Props_in_idx<X> () // v in s ==> s[i] == v
+    ensures forall v: X, s: AbSeq<X> :: AbSeqIn(v, s) ==>
+      (exists i: AbInt :: AbLeqLt(i, I0, AbSeqLen(s)) && AbSeqIndex(i, s) == v )
+    { forall v, s { Seq_Props_in_idx_p2<X>(v, s); } }
+
+  lemma Seq_Props_slice_in_p4<X> (i: AbInt, j: AbInt, s: AbSeq<X>, v: X)
+    ensures AbLeq(I0, i) && AbLeq(j, AbSeqLen(s)) && AbLeq(i, j) ==>
+      AbSeqIn(v, AbSeqSlice(i, j, s)) ==> AbSeqIn(v, s)
+    { }
+  lemma Seq_Props_slice_in<X> ()
+    ensures forall i: AbInt, j: AbInt, s: AbSeq<X>, v: X ::
+      AbLeq(I0, i) && AbLeq(j, AbSeqLen(s)) && AbLeq(i, j) ==>
+      AbSeqIn(v, AbSeqSlice(i, j, s)) ==> AbSeqIn(v, s)
+    { forall i, j, s, v { Seq_Props_slice_in_p4<X>(i, j, s, v); } }
+
+  lemma Seq_Props_index_props ()
+    ensures forall i: AbInt, j: AbInt, x: AbInt, s: AbSeq<AbInt>, s': AbSeq<AbInt> ::
+      ((AbLt(I0, i) || I0 == i) && AbLt(i, AbSeqLen(s)) && AbLt(AbSeqIndex(i, s), x)) ==> 
+      ((AbLt(I0, j) || I0 == j) && AbLt(j, AbSeqLen(s'))) ==>
+      (forall v :: AbSeqIn(v, s') ==> AbSeqIn(v, s)) ==>
+      AbLt(AbSeqIndex(j, s'), x)
+    ensures forall i: AbInt, j: AbInt, x: AbInt, s: AbSeq<AbInt>, s': AbSeq<AbInt> ::
+      ((AbLt(I0, i) || I0 == i) && AbLt(i, AbSeqLen(s)) && AbLt(x, AbSeqIndex(i, s))) ==> 
+      ((AbLt(I0, j) || I0 == j) && AbLt(j, AbSeqLen(s'))) ==>
+      (forall v :: AbSeqIn(v, s') ==> AbSeqIn(v, s)) ==>
+      AbLt(x, AbSeqIndex(j, s'))
+
+}
+
+module ADT_SeqLemma {
+  import opened ADT_Seq`Basic
+
+  lemma Seq_Props_length<X> () // |s| >= 0
+    ensures forall s: AbSeq<X> :: AbLeq(I0, AbSeqLen(s))
+    { forall s { Seq_Props_length_p1<X> (s); } }
+  
+  lemma Seq_Props_concat_length<X> () // |s1 + s2| == |s1| + |s2|
+    ensures forall s1: AbSeq<X>, s2: AbSeq<X> :: AbSeqLen(AbSeqConcat(s1, s2)) == AbAdd(AbSeqLen(s1), AbSeqLen(s2))
+    { forall s1, s2 { Seq_Props_concat_length_p2<X>(s1, s2); } }
+  
+  lemma Seq_Props_concat_in<X> () // x in s1 || x in s2 <==> x in s1 + s2
+    ensures forall x: X, s1: AbSeq<X>, s2: AbSeq<X> :: AbSeqIn(x, s1) || AbSeqIn(x, s2) <==> AbSeqIn(x, AbSeqConcat(s1, s2))
+    { forall x, s1, s2 { Seq_Props_concat_in_p3<X>(x, s1, s2); } }
+  
+  lemma Seq_Props_concat_in_part2all<X> ()
+    // x in s1 ==> x in s1 + s2
+    ensures forall x: X, s1: AbSeq<X>, s2: AbSeq<X> :: AbSeqIn(x, s1) ==> AbSeqIn(x, AbSeqConcat(s1, s2))
+    // x in s2 ==> x in s1 + s2
+    ensures forall x: X, s1: AbSeq<X>, s2: AbSeq<X> :: AbSeqIn(x, s2) ==> AbSeqIn(x, AbSeqConcat(s1, s2))
+    { forall x, s1, s2 { Seq_Props_concat_in_part2all_p3<X>(x, s1, s2); } }
+  
+  lemma Seq_Props_concat_in_all2part<X> ()
+    // x in s1 + s2 && x !in s1 ==> x in s2
+    ensures forall x: X, s1: AbSeq<X>, s2: AbSeq<X> :: AbSeqIn(x, AbSeqConcat(s1, s2)) && !AbSeqIn(x, s1) ==> AbSeqIn(x, s2)
+    // x in s1 + s2 && x !in s2 ==> x in s1
+    ensures forall x: X, s1: AbSeq<X>, s2: AbSeq<X> :: AbSeqIn(x, AbSeqConcat(s1, s2)) && !AbSeqIn(x, s2) ==> AbSeqIn(x, s1)
+    { forall x, s1, s2 { Seq_Props_concat_in_all2part_p3<X>(x, s1, s2); } }
+  
+  lemma Seq_Props_concat_index_part1<X> ()
+    ensures forall i: AbInt, s1: AbSeq<X>, s2: AbSeq<X> ::
+    AbLeqLt(i, I0, AbSeqLen(s1)) ==> // 0 <= i < |s1|
+    AbLt(i, AbSeqLen(AbSeqConcat(s1, s2))) ==> // i < |s1| < |s1 + s2|
+    AbSeqIndex(i, s1) == AbSeqIndex(i, AbSeqConcat(s1, s2))
+    { forall i, s1, s2 { Seq_Props_concat_index_part1_p3<X>(i, s1, s2); } }
+  
+  lemma Seq_Props_concat_index_part2<X> ()
+    ensures forall i: AbInt, s1: AbSeq<X>, s2: AbSeq<X> ::
+      AbLeq(I0, AbAdd(i, AbSeqLen(s1))) ==> // 0 <= i + |s1|
+      (AbLt(i, AbSeqLen(s2)) ==> AbLt(AbAdd(i, AbSeqLen(s1)), AbSeqLen(AbSeqConcat(s1, s2)))) ==> // i + |s1| < |s1 + s2|
+      AbLeqLt(i, I0, AbSeqLen(s2)) ==>
+      AbSeqIndex(i, s2) == AbSeqIndex(AbAdd(i, AbSeqLen(s1)), AbSeqConcat(s1, s2))
+    { forall i, s1, s2 { Seq_Props_concat_index_part2_p3<X>(i, s1, s2); } }
+  
+  lemma Seq_Props_concat_is_orig<X> ()
+    ensures forall i: AbInt, s: AbSeq<X> ::
+      AbLeqLt(i, I0, AbSeqLen(s)) ==> // 0 <= i < |s|
+      s == AbSeqConcat(AbSeqSlice(I0, i, s), AbSeqSlice(i, AbSeqLen(s), s))
+    { forall i, s { Seq_Props_concat_is_orig_p2<X> (i, s); } }
+  
+  lemma Seq_Props_in_empty<X> () // empty seq
+    ensures forall v: X, s: AbSeq<X> :: AbSeqLen(s) == I0 ==> !AbSeqIn(v, s)
+    {forall v, s { Seq_Props_in_empty_p2<X>(v, s); } }
+  
+  lemma Seq_Props_in_non_empty<X> () // i in s ==> |s| > 0
+    ensures forall v: X, s: AbSeq<X> :: AbSeqIn(v, s) ==> AbLt(I0, AbSeqLen(s))
+    {forall v, s { Seq_Props_in_non_empty_p2<X>(v, s); } }
+  
+  lemma Seq_Props_in_idx<X> () // v in s ==> s[i] == v
+    ensures forall v: X, s: AbSeq<X> :: AbSeqIn(v, s) ==>
+      (exists i: AbInt :: AbLeqLt(i, I0, AbSeqLen(s)) && AbSeqIndex(i, s) == v )
+    { forall v, s { Seq_Props_in_idx_p2<X>(v, s); } }
+  
+  lemma Seq_Props_slice_in<X> ()
+    ensures forall i: AbInt, j: AbInt, s: AbSeq<X>, v: X ::
+      AbLeq(I0, i) && AbLeq(j, AbSeqLen(s)) && AbLeq(i, j) ==>
+      AbSeqIn(v, AbSeqSlice(i, j, s)) ==> AbSeqIn(v, s)
+    { forall i, j, s, v { Seq_Props_slice_in_p4<X>(i, j, s, v); } }
+
+}
