SlowTest/SMN-ADT-module-ContLen-Add.dfy
@@ -1,0 +1,464 @@
+// RUN: %dafny /compile:3 "%s" > "%t"
+// RUN: %diff "%s.expect" "%t"
+
+include "ADT-int.dfy"
+datatype List<X> = Nil | Cons(head: X, tail: List<X>)
+
+import opened ADT`Basic
+import opened ADT_Int
+import opened ADT_Set
+
+function method Length(xs: List<AbInt>): AbInt
+{
+  match xs
+  case Nil => I0
+  case Cons(_, tail) => AbAdd(Length(tail), I1)
+}
+ 
+function method Split(xs: List<AbInt>, b: AbInt): (List<AbInt>, List<AbInt>)
+  ensures var r := Split(xs, b); Length(xs) == AbAdd(Length(r.0), Length(r.1))
+  decreases xs
+{
+  Props_add_commutative ();
+  Props_add_associative ();
+  Props_add_identity ();
+  match xs
+  case Nil => (Nil, Nil)
+  case Cons(x, tail) =>
+    var (L, R) := Split(tail, b);
+    if AbLt(x, b) then
+      (Cons(x, L), R)
+    else
+      (L, Cons(x, R))
+}
+
+lemma Split_Correct(xs: List<AbInt>, b: AbInt)
+  requires NoDuplicates(xs)
+  ensures var r := Split(xs, b);
+    Elements(r.0) == (set x | x in Elements(xs) && AbLt(x, b)) && // x < b
+    Elements(r.1) == (set x | x in Elements(xs) && !AbLt(x, b)) && // b <= x
+    NoDuplicates(r.0) && NoDuplicates(r.1)
+{
+  match xs
+  case Nil =>
+  case Cons(_, tail) =>
+    Split_Correct(tail, b);
+}
+
+function Elements(xs: List<AbInt>): set<AbInt>
+{
+  match xs
+  case Nil => {}
+  case Cons(x, tail) => {x} + Elements(tail)
+}
+
+lemma Elements_Property(xs: List<AbInt>)
+  requires NoDuplicates(xs)
+  ensures AbSetLen(Elements(xs)) == Length(xs)
+{
+  Set_Props_len_element();
+  Set_Props_len_empty ();
+  Props_add_associative ();
+}
+
+predicate NoDuplicates(xs: List<AbInt>)
+{
+  match xs
+  case Nil => true
+  case Cons(x, tail) =>
+    x !in Elements(tail) && NoDuplicates(tail)
+}
+
+// standard theorems and their proofs
+
+lemma Cardinality(A: set<AbInt>, B: set<AbInt>)
+  requires A <= B
+  ensures AbLeq(AbSetLen(A), AbSetLen(B))
+{
+  Props_notneg ();
+  Set_Props_len ();
+  Set_Props_len_element ();
+  Set_Props_len_empty ();
+  Props_lt_addition ();
+  Props_add_addition ();
+  Props_add_commutative ();
+  if A != {} {
+    var x :| x in A;
+    Cardinality(A - {x}, B - {x});
+  }
+}
+
+lemma SetEquality(A: set<AbInt>, B: set<AbInt>)
+  requires A <= B && AbSetLen(A) == AbSetLen(B)
+  ensures A == B
+{
+  Set_Props_len ();
+  Set_Props_len_element ();
+  Set_Props_len_empty ();
+  Props_add_addition ();
+  if A == {} {
+  } else {
+    var x :| x in A;
+    SetEquality(A - {x}, B - {x});
+  }
+}
+
+function IntRange(lo: AbInt, len: AbInt): set<AbInt>
+  ensures AbSetLen(IntRange(lo, len)) == len
+{
+  Props_add2sub ();
+  Props_add_sub_is_orig ();
+  var S := AbBoundSet(lo, AbAdd(lo, len));
+  // Try not to assign every element with AbAdd()
+  // assert len != 0 ==> S == IntRange(lo, len - 1) + {AbAdd(lo, I2A(len - 1))};
+  assert forall x :: (AbLeq(lo, x) && AbLt(x, AbAdd(lo, len))) ==> x in S;
+  S
+}
+
+function method SmallestMissingNumber(xs: List<AbInt>): AbInt
+{
+  SMN(xs, I0, Length(xs))
+}
+
+function method SMN(xs: List<AbInt>, n: AbInt, len: AbInt): AbInt
+  requires len == Length(xs)
+  decreases A2D(len)
+{
+  Props_add_commutative ();
+  if AbLeq(I2, len) then
+    var (L, R) := Split(xs, AbAdd(n, AbDiv2(len)));
+    var llen := Length(L);
+
+    if AbLt(llen, AbDiv2(len)) then
+      // len / 2 < len
+      Props_pos(I2); // I0 < I2
+      Props_lt_transitive (); // I0 < I2 < len
+      Props_div_lt (); // x >= 2 ==> x / 2 < x
+      Props_adt_dt_lt (llen, len);
+      SMN(L, n, llen)
+    else
+      Props_lt_gt_eq_p2 (llen, AbDiv2(len));
+      // 0 < len / 2
+      Props_div_pos2 (); // x >= 2 ==> x / 2 > 0
+      Props_lt_transitive (); // 0 < len / 2 < llen
+      Props_add2sub ();
+      Props_add_pos_is_lt ();
+      Props_adt_dt_lt (AbSub(len, llen), len);
+      SMN(R, AbAdd(n, llen), AbSub(len, llen))
+  else if xs.Cons? then
+    if xs.head == n then AbAdd(n, I1) else n
+  else
+    n
+}
+
+// proof of lemmas supporting proof of main theorem
+
+lemma SmallestMissingNumber_Correct(xs: List<AbInt>)
+  requires NoDuplicates(xs)
+  ensures var s := SmallestMissingNumber(xs);
+    s !in Elements(xs) &&
+    forall x :: AbLeqLt(x, I0, s) ==> x in Elements(xs)
+{
+  forall x | x in Elements(xs)
+    ensures AbLeq(I0, x)
+    { Props_notneg(); }
+  SMN_Correct(xs, I0, Length(xs));
+}
+
+// element, len, index -> abstract type
+lemma SMN_Correct(xs: List<AbInt>, n: AbInt, len: AbInt)
+  requires NoDuplicates(xs)
+  requires forall x :: x in Elements(xs) ==> AbLeq(n, x)
+  requires len == Length(xs)
+  ensures var s := SMN(xs, n, len);
+    AbLeq(n, s) &&
+    AbLeq(s, AbAdd(n, len)) &&
+    s !in Elements(xs) &&
+    forall x :: AbLeqLt(x, n, s) ==> x in Elements(xs)
+  decreases A2D(len)
+{
+  Props_notneg();
+  Props_add_commutative ();
+  if AbLeq(I2, len) {
+    var (L, R) := Split(xs, AbAdd(n, AbDiv2(len)));
+    Split_Correct(xs, AbAdd(n, AbDiv2(len)));
+    var llen := Length(L);
+    Elements_Property(L);  // NoDuplicates property
+    var bound := IntRange(n, AbDiv2(len));
+    Cardinality(Elements(L), bound);
+    
+    if AbLt(llen, AbDiv2(len)) {
+      var s := SMN(L, n, llen);
+      // len / 2 < len
+      Props_pos(I2); // I0 < I2
+      Props_lt_transitive (); // I0 < I2 < len
+      Props_div_lt (); // x >= 2 ==> x / 2 < x
+      Props_adt_dt_lt (llen, len); // decreases (pre: llen < len/2 < len)
+      SMN_Correct(L, n, llen);
+
+      Props_lt_addition (); // a < b ==> x + a < x + b: Lt(s, n+llen) ==> Lt(s, n+len)
+      Props_add_lt_is_lt_p4(s, n, llen, len); // x = y + a && a < b ==> x < y + b: s==n+llen ==> Lt(s, n+len)
+    } else {
+      // 0 < len / 2
+      Props_div_pos2 (); // x >= 2 ==> x / 2 > 0
+      Props_lt_transitive (); // 0 < len / 2 < llen
+      Props_add2sub ();
+      Props_add_pos_is_lt ();
+      Props_adt_dt_lt (AbSub(len, llen), len);
+      var s := SMN(R, AbAdd(n, llen), AbSub(len, llen));
+      Props_lt_gt_eq_py (AbAdd(n, llen));
+      SMN_Correct(R, AbAdd(n, llen), AbSub(len, llen));
+
+      Props_add_notneg_is_leq (); // x + a == y ==> x < y || x == y: n+llen == s ==> Lt(n, s)
+      Props_add_sub_is_add_p3(n, len, llen); // no trigger loop
+      forall x | (AbLt(n, x) || n == x) && AbLt(x, s)
+        ensures x in Elements(xs)
+      {
+        if AbLt(x, AbAdd(n, llen)) {
+          SetEquality(Elements(L), bound);
+        }
+      }
+    }
+  } 
+  else if xs.Cons? {
+    Props_pos(I1); // 0 < 1
+    Props_2is1add1 ();
+    Props_lt_gt_eq ();
+    Props_one_in_bound_p2 (I1, len);
+    Props_add_notneg_is_leq (); // x + a == y ==> x <= y
+    Props_add_pos_is_lt (); // x < x + Positive
+    if xs.head == n {
+      Props_add_identity ();
+      Props_one_in_bound ();
+    } else { }
+  } else {
+    Props_lt_gt_eq ();
+    Props_add_identity ();
+  }
+}
+
+function method SMN'(xs: List<AbInt>, n: AbInt, len: AbInt): AbInt
+  requires len == Length(xs)
+  decreases A2D(len)
+{
+  if xs == Nil then n
+  else
+    var half := AbDiv2(AbAdd(len, I1)); // half = (len+1)/2
+    var (L, R) := Split(xs, AbAdd(n, half));
+    var llen := Length(L);
+    if AbLt(llen, half) then
+      Props_pos(I1); // 0 < 1
+      Props_notneg ();
+      Props_add_identity ();
+      Props_add_pos_is_pos (); // x + Positive = Positive
+      Props_lt2leq_p2 (I0, len); // len > 0 ==> len >= 1
+      Props_div_leq_p2 (len, I1);  // len >= 1 ==> (len+1)/2 <= len
+      Props_lt_transitive (); // llen < (len+1)/2 < len
+      Props_adt_dt_lt (llen, len);
+      SMN'(L, n, llen)
+    else
+      Props_pos(I1); // 0 < 1
+      Props_notneg ();
+      Props_add_identity ();
+      Props_add_pos_is_pos (); // x + Positive = Positive
+      Props_lt2leq_p2 (I0, len); // len > 0 ==> len >= 1
+      Props_div_pos1 (); // (len+1)/2 > 0
+      Props_lt_transitive (); // 0 < (len+1)/2 < llen
+      Props_add_sub_is_orig ();
+      Props_add_pos_is_lt ();
+      Props_adt_dt_lt (AbSub(len, llen), len);
+      Props_add2sub ();
+      SMN'(R, AbAdd(n, llen), AbSub(len, llen))
+}
+
+lemma SMN'_Correct(xs: List<AbInt>, n: AbInt, len: AbInt)
+  requires NoDuplicates(xs)
+  requires forall x :: x in Elements(xs) ==> AbLeq(n, x)
+  requires len == Length(xs)
+  ensures var s := SMN'(xs, n, len);
+    AbLeq(n, s) &&
+    AbLeq(s, AbAdd(n, len)) &&
+    s !in Elements(xs) &&
+    forall x :: AbLeqLt(x, n, s) ==> x in Elements(xs)
+  decreases A2D(len)
+{
+  Props_add_commutative ();
+  if xs == Nil {
+    Props_add_identity ();
+    Props_lt_gt_eq ();
+  } else {
+    var half := AbDiv2(AbAdd(len, I1)); // half = (len+1)/2
+    var (L, R) := Split(xs, AbAdd(n, half));
+    Split_Correct(xs, AbAdd(n, half));
+    var llen := Length(L);
+    Elements_Property(L);  // use the NoDuplicates property
+    var bound := IntRange(n, half);
+    Cardinality(Elements(L), bound);
+    if AbLt(llen, half) {
+      var s := SMN'(L, n, llen);
+      Props_pos(I1); // 0 < 1
+      Props_notneg();
+      Props_add_identity ();
+      Props_add_pos_is_pos (); // x + Positive = Positive
+      Props_lt2leq_p2 (I0, len); // len > 0 ==> len >= 1
+      Props_div_leq_p2 (len, I1);  // len >= 1 ==> (len+1)/2 <= len
+      Props_lt_transitive (); // llen < (len+1)/2 < len
+      Props_adt_dt_lt (llen, len);
+      SMN'_Correct(L, n, llen);
+
+      Props_lt_addition (); // a < b ==> x + a < x + b: Lt(s, n+llen) ==> Lt(s, n+len)
+      Props_add_lt_is_lt_p4(s, n, llen, len); // x = y + a && a < b ==> x < y + b: s==n+llen ==> Lt(s, n+len)
+    } else {
+      Props_pos(I1); // 0 < 1
+      Props_notneg();
+      Props_add_identity ();
+      Props_add_pos_is_pos (); // x + Positive = Positive
+      Props_lt2leq_p2 (I0, len); // len > 0 ==> len >= 1
+      Props_div_pos1 (); // (len+1)/2 > 0
+      Props_lt_transitive (); // 0 < (len+1)/2 < llen
+      Props_add_sub_is_orig ();
+      Props_add_pos_is_lt ();
+      Props_adt_dt_lt (AbSub(len, llen), len);
+      Props_add2sub ();
+      var s := SMN'(R, AbAdd(n, llen), AbSub(len, llen));
+      Props_lt_gt_eq_py (AbAdd(n, llen));
+      SMN'_Correct(R, AbAdd(n, llen), AbSub(len, llen));
+
+      Props_add_sub_is_add_p3(n, len, llen); // no trigger loop
+      forall x | (AbLt(n, x) || n == x) && AbLt(x, s)
+        ensures x in Elements(xs)
+      {
+        if AbLt(x, AbAdd(n, llen)) {
+          SetEquality(Elements(L), bound);
+        }
+      }
+    }
+  }
+}
+
+function method SMN''(xs: List<AbInt>, n: AbInt, len: AbInt): AbInt
+  requires len == Length(xs)
+  decreases A2D(len)
+{
+  if xs == Nil then n
+  else
+    var half := AbAdd(AbDiv2(len), I1); // half = len/2 + 1
+    var (L, R) := Split(xs, AbAdd(n, half));
+    var llen := Length(L);
+    if AbLt(llen, half) then
+      Props_pos(I1); // 0 < 1
+      Props_notneg ();
+      Props_add_identity ();
+      Props_add_pos_is_pos (); // x + Positive = Positive
+      Props_lt2leq_p2 (I0, len); // len > 0 ==> len >= 1
+      Props_div_add1_leq_p1 (len);
+      Props_lt_transitive ();
+      Props_adt_dt_lt (llen, len);
+      SMN''(L, n, llen)
+    else
+      Props_pos(I1); // 0 < 1
+      Props_notneg ();
+      Props_add_identity ();
+      Props_add_pos_is_pos (); // x + Positive = Positive
+      Props_lt2leq_p2 (I0, len); // len > 0 ==> len >= 1
+      Props_add_pos_is_lt (); // x < x + Positive
+      Props_lt_transitive (); // len/2 + 1 > 0
+      Props_add_sub_is_orig ();
+      Props_adt_dt_lt (AbSub(len, llen), len);
+      Props_add2sub ();
+      SMN''(R, AbAdd(n, llen), AbSub(len, llen))
+}
+
+lemma SMN''_Correct(xs: List<AbInt>, n: AbInt, len: AbInt)
+  requires NoDuplicates(xs)
+  requires forall x :: x in Elements(xs) ==> AbLeq(n, x)
+  requires len == Length(xs)
+  ensures var s := SMN''(xs, n, len);
+    AbLeq(n, s) &&
+    AbLeq(s, AbAdd(n, len)) &&
+    s !in Elements(xs) &&
+    forall x :: AbLeqLt(x, n, s) ==> x in Elements(xs)
+  decreases A2D(len)
+{
+  Props_add_commutative ();
+  if xs == Nil {
+    Props_lt_gt_eq (); // x < y <==> !x > y && x != y
+    Props_add_identity ();
+  } else {
+    var half := AbAdd(AbDiv2(len), I1); // half = len/2 + 1
+    var (L, R) := Split(xs, AbAdd(n, half));
+    Split_Correct(xs, AbAdd(n, half));
+    var llen := Length(L);
+    Elements_Property(L);  // use the NoDuplicates property
+    var bound := IntRange(n, half);
+    Cardinality(Elements(L), bound);
+    if AbLt(llen, half) {
+      var s := SMN''(L, n, llen);
+      Props_pos(I1); // 0 < 1
+      Props_notneg ();
+      Props_add_identity ();
+      Props_add_pos_is_pos (); // x + Positive = Positive
+      Props_lt2leq_p2 (I0, len); // len > 0 ==> len >= 1
+      Props_div_add1_leq_p1 (len);
+      Props_lt_transitive ();
+      Props_adt_dt_lt (llen, len);
+      SMN''_Correct(L, n, llen);
+
+      Props_lt_addition (); // a < b ==> x + a < x + b: Lt(s, n+llen) ==> Lt(s, n+len)
+      Props_add_lt_is_lt_p4(s, n, llen, len); // x = y + a && a < b ==> x < y + b: s==n+llen ==> Lt(s, n+len)
+    } else {
+      Props_pos(I1); // 0 < 1
+      Props_notneg ();
+      Props_add_identity ();
+      Props_add_pos_is_pos (); // x + Positive = Positive
+      Props_lt2leq_p2 (I0, len); // len > 0 ==> len >= 1
+      Props_add_pos_is_lt (); // x < x + Positive
+      Props_lt_transitive (); // len/2 + 1 > 0
+      Props_add_sub_is_orig ();
+      Props_adt_dt_lt (AbSub(len, llen), len);
+      Props_add2sub ();
+      var s := SMN''(R, AbAdd(n, llen), AbSub(len, llen));
+      Props_lt_gt_eq_py (AbAdd(n, llen));
+      SMN''_Correct(R, AbAdd(n, llen), AbSub(len, llen));
+
+      Props_add_sub_is_add_p3(n, len, llen); // no trigger loop
+      forall x | (AbLt(n, x) || n == x) && AbLt(x, s)
+        ensures x in Elements(xs)
+      {
+        if AbLt(x, AbAdd(n, llen)) {
+          SetEquality(Elements(L), bound);
+        }
+      }
+    }
+  }
+}
+
+// // TODO: need more concrete props to make it verified.
+// method Main() {
+//   var xs := Nil;
+//   assert Length(xs) == I0;
+//   var s := SmallestMissingNumber(xs);
+//   Props_notneg ();
+//   Props_add_associative ();
+//   Props_add_identity ();
+//   Props_add_commutative ();
+//   Props_add_pos_is_pos ();
+//   Props_pos(I2);
+//   Props_lt_transitive ();
+//   Props_lt_gt_eq ();
+//   assert s == I0;
+//   print s, " ";  // 0
+//   var a := Cons(I2, Cons(I0, Nil));
+//   Props_2is1add1 ();
+//   assume I1 == AbDiv2(I2);
+//   assume AbLt(I0, I1);
+//   assume AbLt(I1, I2);
+//   // assert SmallestMissingNumbxer(a) == I1;
+//   // print SmallestMissingNumber(a), " ";  // 1
+//   a := Cons(I2A(3), Cons(I1, a));
+//   // assert SmallestMissingNumber(a) == I2A(4);
+// //   print SmallestMissingNumber(a), " ";  // 4
+//   a := Cons(I2A(7), Cons(I2A(4), Cons(I2A(6), a)));
+//   // assert SmallestMissingNumber(a) == I2A(5);
+// //   print SmallestMissingNumber(a), "\n";  // 5
+// }
